progs/verif_sort.v
@@ -1,0 +1,47 @@
+Require Import floyd.proofauto.
+Require Import progs.list_dt.
+Require Import progs.sort.
+Require Import Sorted.
+Require Import Omega.
+Require Import Coq.Sorting.Permutation.
+
+Local Open Scope logic.
+
+Instance CompSpecs : compspecs. make_compspecs prog. Defined.
+Definition Vprog : varspecs. mk_varspecs prog. Defined.
+
+Definition apply_spec :=
+Definition spawn_spec :=
+  WITH f : val,
+       b : val,
+       PrePost :
+         { ty : Type &
+          (ty *                     (* WITH clause for spawned function *)
+          (ty -> val -> Pred))%type}  (* precondition (postcondition is emp) *)
+   PRE [_f OF tptr voidstar_funtype, _args OF tptr tvoid]
+     PROP ( )
+     LOCAL (temp _args b)
+     SEP
+     (match PrePost with existT ty (_, pre) =>
+      EX _y : ident, EX globals : ty -> list (ident * val),
+      (func_ptr'
+        (WITH y : val, x : ty
+          PRE [ _y OF tptr tvoid ]
+            PROP ()
+            (LOCALx (temp _y y :: map (fun x => gvar (fst x) (snd x)) (globals x))
+            (SEP   (Interp (pre x y))))
+          POST [tptr tvoid]
+            PROP  ()
+            LOCAL ()
+            SEP   (emp))
+       f)
+      end;
+        match PrePost with
+          existT ty (w, pre) =>
+          Interp (pre w b)
+      end
+     )
+   POST [ tvoid  ]
+     PROP  ()
+     LOCAL ()
+     SEP   (emp).
